theories/Interp.v
@@ -23,13 +23,13 @@ End Env.
 
 Notation "κ ∷ σ" := (Env.cons κ σ) (at level 30).
 
-Reserved Notation "⟦ e ⟧ κs" (at level 50).
+Reserved Notation "⟦ M ⟧ κs" (at level 50).
 
-Fixpoint interp_tm `(e : EProg.t Λ Ψ) (κs : Env.t Λ) : Prog.t Ψ :=
-  match e with
+Fixpoint interp_tm `(M : EProg.t Λ Ψ) (κs : Env.t Λ) : Prog.t Ψ :=
+  match M with
   | EProg.var i => Prog.var i
-  | EProg.fst e => ⟦e⟧ κs .1
-  | EProg.snd e => ⟦e⟧ κs .2
+  | EProg.fst M => ⟦M⟧ κs .1
+  | EProg.snd M => ⟦M⟧ κs .2
   | EProg.unit => 𝟙
   | EProg.bool => 𝟚
   | EProg.ax => ★
@@ -41,13 +41,13 @@ Fixpoint interp_tm `(e : EProg.t Λ Ψ) (κs : Env.t Λ) : Prog.t Ψ :=
   | EProg.ltr r A => ▶[κs r] ⟦A⟧ κs
   | EProg.isect A => ⋂[κ] ⟦A⟧ κ ∷ κs
   | EProg.univ i => 𝕌[i]
-  | EProg.fix_ e => 𝛍{⟦e⟧ κs}
-  | EProg.lam e => 𝛌{⟦e⟧ κs}
-  | EProg.app e1 e2 => ⟦e1⟧ κs ⋅ ⟦e2⟧ κs
+  | EProg.fix_ M => 𝛍{⟦M⟧ κs}
+  | EProg.lam M => 𝛌{⟦M⟧ κs}
+  | EProg.app M1 M2 => ⟦M1⟧ κs ⋅ ⟦M2⟧ κs
   end
-where "⟦ e ⟧ κs" := (interp_tm e%etm κs) : prog_scope.
+where "⟦ M ⟧ κs" := (interp_tm M%etm κs) : prog_scope.
 
-Arguments interp_tm [Λ Ψ] e%etm κs.
+Arguments interp_tm [Λ Ψ] M%etm κs.
 
 Program Fixpoint interp_ctx `(Γ : ECtx.t Λ Ψ) (κs : Env.t Λ) : Prectx Ψ :=
   match Γ with
@@ -61,12 +61,12 @@ Arguments interp_ctx [Λ Ψ] Γ%ectx κs.
 Definition interp_jdg `(J : EJdg.t Λ) : Ω :=
   ∀ κs,
     match J with
-    | ⌊ _ ∣ Γ ≫ A ∋ e1 ≐ e2 ⌋ =>
+    | ⌊ _ ∣ Γ ≫ A ∋ M1 ≐ M2 ⌋ =>
       τω ⊧ ⟦ Γ ⟧ κs ctx
       → (τω ⊧ ⟦ Γ ⟧ κs ≫ ⟦ A ⟧ κs ∼ ⟦ A ⟧ κs)
-      → τω ⊧ ⟦ Γ ⟧ κs ≫ ⟦ A ⟧ κs ∋ ⟦ e1 ⟧ κs ∼ ⟦ e2 ⟧ κs
-    | ⌊ _ ∣ Ψ ⊢ e1 ≃ e2 ⌋ =>
-      (⟦ e1 ⟧ κs) ≈ (⟦ e2 ⟧ κs)
+      → τω ⊧ ⟦ Γ ⟧ κs ≫ ⟦ A ⟧ κs ∋ ⟦ M1 ⟧ κs ∼ ⟦ M2 ⟧ κs
+    | ⌊ _ ∣ Ψ ⊢ M1 ≃ M2 ⌋ =>
+      (⟦ M1 ⟧ κs) ≈ (⟦ M2 ⟧ κs)
     end.
 
 Arguments interp_jdg [Λ] J%ejdg.
@@ -82,10 +82,10 @@ Notation "⟦ σ ⟧ κs" := (interp_subst σ%esubst κs) : subst_scope.
 Local Open Scope prog_scope.
 Local Open Scope program_scope.
 
-Theorem interp_tm_clk_naturality {Λ1 Λ2 Ψ} (e : EProg.t Λ1 Ψ) (ρ : Ren.t Λ1 Λ2) (κs : Env.t Λ2) :
-  ⟦ e ⟧ κs ∘ ρ = ⟦ e.⦃ρ⦄ ⟧ κs.
+Theorem interp_tm_clk_naturality {Λ1 Λ2 Ψ} (M : EProg.t Λ1 Ψ) (ρ : Ren.t Λ1 Λ2) (κs : Env.t Λ2) :
+  ⟦ M ⟧ κs ∘ ρ = ⟦ M.⦃ρ⦄ ⟧ κs.
 Proof.
-  move: Λ2 ρ κs; elim e => *;
+  move: Λ2 ρ κs; elim M => *;
   T.rewrites_with ltac:(try rewrite Ren.cong_id).
 
   repeat f_equal; T.eqcd => *.
@@ -106,11 +106,11 @@ Proof.
   T.rewrites.
 Qed.
 
-Theorem interp_tm_var_naturality {Λ Ψ0 Ψ1 Ψ2} (e : EProg.t Λ Ψ0) (σ : Sub.t Ψ1 Ψ2) ρ κs :
-  (⟦ e ⟧ κs) ⫽ (σ ∘ ρ) = (⟦ e.[ρ] ⟧ κs) ⫽ σ.
+Theorem interp_tm_var_naturality {Λ Ψ0 Ψ1 Ψ2} (M : EProg.t Λ Ψ0) (σ : Sub.t Ψ1 Ψ2) ρ κs :
+  (⟦ M ⟧ κs) ⫽ (σ ∘ ρ) = (⟦ M.[ρ] ⟧ κs) ⫽ σ.
 Proof.
   move: Ψ1 Ψ2 σ ρ κs.
-  induction e; eauto; simpl;
+  induction M; eauto; simpl;
   T.rewrites_with
     ltac:(repeat f_equal;
           try (T.eqcd; intros);
@@ -119,12 +119,12 @@ Proof.
 Qed.
 
 
-Theorem interp_tm_var_ren_naturality {Λ Ψ0 Ψ1} (e : EProg.t Λ Ψ0) (ρ : Ren.t Ψ0 Ψ1) κs :
-  (⟦ e ⟧ κs).[ ρ ] = (⟦ e.[ρ] ⟧ κs).
+Theorem interp_tm_var_ren_naturality {Λ Ψ0 Ψ1} (M : EProg.t Λ Ψ0) (ρ : Ren.t Ψ0 Ψ1) κs :
+  (⟦ M ⟧ κs).[ ρ ] = (⟦ M.[ρ] ⟧ κs).
 Proof.
   by rewrite
-     -(Prog.subst_ret (⟦ e .[ ρ] ⟧ κs))
-     -(Prog.subst_ret (⟦ e ⟧ κs .[ρ]))
+     -(Prog.subst_ret (⟦ M .[ ρ] ⟧ κs))
+     -(Prog.subst_ret (⟦ M ⟧ κs .[ρ]))
      Prog.subst_ren_coh
      interp_tm_var_naturality.
 Qed.
@@ -141,12 +141,12 @@ Proof.
     by rewrite -interp_tm_var_naturality.
 Qed.
 
-Theorem interp_tm_subst_naturality {Λ Ψ0 Ψ1 Ψ2} (e : EProg.t Λ Ψ0) (σ12 : Sub.t Ψ1 Ψ2) (σ01 : Sub.t Ψ0 Ψ1) κs :
-  (⟦ e ⟧ κs) ⫽ (σ12 ◎ ⟦ σ01 ⟧ κs) = (⟦ e ⫽ σ01 ⟧ κs) ⫽ σ12.
+Theorem interp_tm_subst_naturality {Λ Ψ0 Ψ1 Ψ2} (M : EProg.t Λ Ψ0) (σ12 : Sub.t Ψ1 Ψ2) (σ01 : Sub.t Ψ0 Ψ1) κs :
+  (⟦ M ⟧ κs) ⫽ (σ12 ◎ ⟦ σ01 ⟧ κs) = (⟦ M ⫽ σ01 ⟧ κs) ⫽ σ12.
 Proof.
   symmetry.
   move: Ψ1 Ψ2 σ01 σ12 κs.
-  induction e; eauto; simpl;
+  induction M; eauto; simpl;
   T.rewrites_with
     ltac:(repeat f_equal; try (T.eqcd; intros);
           try rewrite /interp_subst /EProg.wk_sub;
@@ -155,12 +155,12 @@ Proof.
           try rewrite -interp_tm_clk_naturality).
 Qed.
 
-Theorem interp_tm_ren_naturality {Λ0 Λ1 Ψ0 Ψ1 Ψ2} (e : EProg.t Λ0 Ψ0) (ρΛ : Ren.t Λ0 Λ1) (ρΨ : Ren.t Ψ0 Ψ1) (σ : Sub.t Ψ1 Ψ2) κs :
-  (⟦ e ⟧ κs ∘ ρΛ) ⫽ (σ ∘ ρΨ) = (⟦ e.⦃ρΛ⦄[ρΨ] ⟧ κs) ⫽ σ.
+Theorem interp_tm_ren_naturality {Λ0 Λ1 Ψ0 Ψ1 Ψ2} (M : EProg.t Λ0 Ψ0) (ρΛ : Ren.t Λ0 Λ1) (ρΨ : Ren.t Ψ0 Ψ1) (σ : Sub.t Ψ1 Ψ2) κs :
+  (⟦ M ⟧ κs ∘ ρΛ) ⫽ (σ ∘ ρΨ) = (⟦ M.⦃ρΛ⦄[ρΨ] ⟧ κs) ⫽ σ.
 Proof.
   symmetry.
   move: Ψ1 Ψ2 σ Λ1 ρΨ ρΛ κs.
-  induction e; eauto; simpl;
+  induction M; eauto; simpl;
 
   T.rewrites_with
     ltac:(repeat f_equal; try (T.eqcd; intros);
